@prefix : <https://w3id.org/faia/ont/> .
@prefix owl: <http://www.w3.org/2002/07/owl#> .
@prefix rdf: <http://www.w3.org/1999/02/22-rdf-syntax-ns#> .
@prefix xml: <http://www.w3.org/XML/1998/namespace> .
@prefix xsd: <http://www.w3.org/2001/XMLSchema#> .
@prefix faia: <https://w3id.org/faia/ont/> .
@prefix rdfs: <http://www.w3.org/2000/01/rdf-schema#> .
@base <https://w3id.org/faia/ont/> .

<https://w3id.org/faia/ont/> rdf:type owl:Ontology ;
                              owl:versionIRI <https://w3id.org/faia/ont/1.0.0> ;
                              owl:imports <https://w3id.org/liccium/ont/> .

#################################################################
#    Data properties
#################################################################

###  https://w3id.org/faia/ont/AImodel
faia:AImodel rdf:type owl:DatatypeProperty ;
             rdfs:domain <https://w3id.org/liccium/ont/Declaration> ;
             rdfs:range xsd:string ;
             rdfs:comment "Specific AI model identifier or name used by the tool." ;
             rdfs:label "AI model" .


###  https://w3id.org/faia/ont/activityCode
faia:activityCode rdf:type owl:DatatypeProperty ;
                  rdfs:domain <https://w3id.org/liccium/ont/Declaration> ;
                  rdfs:range xsd:anyURI ;
                  rdfs:comment "Code describing the activity or workflow step, aligned with FAIA or STM AI classification." ;
                  rdfs:label "activity code" .


###  https://w3id.org/faia/ont/faiaFlag
faia:faiaFlag rdf:type owl:DatatypeProperty ;
              rdfs:domain <https://w3id.org/liccium/ont/Declaration> ;
              rdfs:range xsd:anyURI ;
              rdfs:comment "Indicates AI involvement in the creation or modification of the work, according to the FAIA classification." ;
              rdfs:label "FAIA flag" .


###  https://w3id.org/faia/ont/tool
<https://w3id.org/faia/ont/tool> rdf:type owl:DatatypeProperty ;
                                  rdfs:domain <https://w3id.org/liccium/ont/Declaration> ;
                                  rdfs:range xsd:string ;
                                  rdfs:comment "Name of the AI tool or software used in generating or modifying the content" ;
                                  rdfs:label "tool" .


#################################################################
#    Classes
#################################################################

###  https://w3id.org/liccium/ont/Declaration
<https://w3id.org/liccium/ont/Declaration> rdf:type owl:Class .


###  Generated by the OWL API (version 4.5.29.2024-05-13T12:11:03Z) https://github.com/owlcs/owlapi
